working on SepExpr, reconsidering the need for unification variables...

src/SepTheoryX.v
@@ -1,7 +1,7 @@
 Require Import Heaps.
-Require Import PropX.
+Require Import PropX PropXTac.
 Require Import Env.
-Require Import PropXTac.
+Require Import IL.
 
 Require Import RelationClasses.
 
@@ -15,62 +15,36 @@ Module SepTheoryX (H : Heap).
     Variable pcType : Type.    
     Variable stateType : Type.
 
-    Definition hprop (sos : list Type) := HT.smem -> propX pcType stateType sos.
+    Definition hprop (sos : list Type) := settings -> HT.smem -> propX pcType stateType sos.
 
     Variable cs : codeSpec pcType stateType.
-    Require Import List.
-    
-    Fixpoint forallXify (ls : list Type) : propX pcType stateType ls -> PropX pcType stateType :=
-      match ls with
-        | nil => fun x => x 
-        | a :: b => fun x => forallXify (PropX.ForallX x)
-      end.
-
-    Fixpoint SubstAll dom (m : hlist (fun T => T -> PropX pcType stateType) dom) (p : propX pcType stateType dom) : PropX pcType stateType :=
-      match p in propX _ _ dom 
-        return hlist (fun T => T -> PropX pcType stateType) dom -> PropX pcType stateType
-        with 
-        | Inj _ p => fun _ => Inj p
-        | Cptr _ pc s => fun m => Cptr pc (fun x => SubstAll m (s x))
-        | And _ l r => fun m => And (SubstAll m l) (SubstAll m r)
-        | Or _ l r => fun m => Or (SubstAll m l) (SubstAll m r)
-        | Imply _ l r => fun m => Imply (SubstAll m l) (SubstAll m r)
-
-        | _ => fun _ => Inj True
-      end m.
-
-    Lemma forallXify_subst : forall sos (l : propX pcType stateType sos),
-      (forall m : hlist (fun T => T -> PropX pcType stateType) sos, 
-        interp cs (SubstAll m l))
-      -> interp cs (forallXify l).
-    Admitted.
 
     Definition himp (gl gr : hprop nil) : Prop :=
-      forall m, interp cs (gl m --> gr m).
+      forall s m, interp cs (gl s m) -> interp cs (gr s m).
     Definition heq (gl gr : hprop nil) : Prop :=
       himp gl gr /\ himp gr gl.
 
-    Global Instance Relf_himp : Reflexive himp.
+    Global Instance Refl_himp : Reflexive himp.
     Proof.
-      red. unfold himp. intros. apply Imply_I. econstructor; simpl; auto.
+      red; unfold himp; firstorder.
     Qed.
     Global Instance Trans_himp : Transitive himp.
     Proof.
-      red. unfold himp. firstorder. apply Imply_I.
-    Admitted.
+      red; unfold himp; firstorder.
+    Qed.
 
-    Global Instance Relf_heq : Reflexive heq.
+    Global Instance Refl_heq : Reflexive heq.
     Proof.
-      red. unfold heq. 
-    Admitted.
+      red; unfold heq; auto; split; reflexivity.
+    Qed.
     Global Instance Sym_heq : Symmetric heq.
     Proof.
-      red. unfold heq. 
-    Admitted.
+      red; unfold heq; firstorder.
+    Qed.
     Global Instance Trans_heq : Transitive heq.
     Proof.
-      red. unfold heq.
-    Admitted.
+      red; unfold heq; firstorder.
+    Qed.
 
     Theorem heq_himp : forall a b, heq a b -> himp a b.
     Proof.
@@ -82,148 +56,55 @@ Module SepTheoryX (H : Heap).
       unfold heq; firstorder.
     Qed.
 
-    Require Import PropXTac.
-    Ltac goPropX := 
-      repeat match goal with
-               | [ H : valid _ _ _ |- _ ] => apply simplify_fwd in H; simpl in H
-               | [ |- valid _ _ _ ] => apply simplify_bwd; simpl
-               | [ H : exists x , _ |- _ ] => destruct H
-               | [ H : _ /\ _ |- _ ] => destruct H
-             end.
+    (* Definitions *)
+    Definition inj sos (p : propX pcType stateType sos) : hprop sos :=
+      fun _ m => PropX.And p (PropX.Inj (HT.semp m)).
+
+    Definition emp {sos} : hprop sos := inj (PropX.Inj True).
+
+    Definition star sos (l r : hprop sos) : hprop sos :=
+      fun s m => PropX.Exists (fun ml : HT.smem => PropX.Exists (fun mr : HT.smem =>
+        PropX.And (PropX.Inj (HT.split m ml mr)) (And (l s ml) (r s mr)))).
+
+    Definition ex sos (T : Type) (p : T -> hprop sos) : hprop sos :=
+      fun s h => PropX.Exists (fun t => p t s h).
+
+    Definition hptsto sos (p : H.addr) (v : H.byte) : hprop sos :=
+      fun s h => 
+        PropX.Inj (HT.smem_get p h = Some v /\ forall p', p' <> p -> HT.smem_get p' h = None).
+
+    (** Lemmas **)
     Ltac doIt :=
       unfold himp, heq; simpl; intros;
         repeat match goal with
-                 | [ h : HT.smem , H : forall x : HT.smem , _ |- _ ] => specialize (H h)
+(*                 | [ h : HT.smem , H : forall x : HT.smem , _ |- _ ] => specialize (H h) *)
                  | [ H : _ -> _ |- _ ] => apply H; clear H
+                 | [ H : forall x, _ -> _ , H' : _ |- _ ] => apply H in H'
                  | [ H : ?X -> _ , H' : ?X |- _ ] => apply H in H'; clear H
-               end; goPropX;
+               end; propxFo;
         repeat match goal with
                  | [ |- exists x, _ ] => eexists
                  | [ |- _ /\ _ ] => split
-                 | [ |- simplify _ _ _ ] => eassumption
+                 | [ |- simplify _ _ _ ] => eassumption || apply simplify_fwd
+                 | [ H : interp ?X (?Y _) |- interp ?X (?Y _) ] => eapply H
                end.
 
-    (* Definitions *)
-    Definition inj sos (p : propX pcType stateType sos) : hprop sos :=
-      fun m => PropX.And p (PropX.Inj (HT.semp m)).
-(*    
-    Theorem hinj_respects (p : PropX pcType stateType) : forall cs G m m', 
-      HT.smem_eq m m' -> valid cs G ((hinj p) m --> (hinj p) m').
-    Proof.
-      unfold hinj; intros. eapply Imply_I. eapply And_I.
-      eapply And_E1. econstructor; left; reflexivity.
-      unfold emp, hemp in *. simpl in *. eapply Inj_E. eapply And_E2.
-      econstructor; left; reflexivity. intros; eapply Inj_I. 
-      eapply HT.semp_mor; eauto. symmetry; eassumption. 
-    Qed.
-
-    Definition inj (p : PropX pcType stateType) : Hprop := Build_Hprop _ (hinj_respects p).
-*)
-
-    Definition emp {sos} : hprop sos := inj (PropX.Inj True).
-(*
-    Theorem hemp_respects : forall cs G m m', HT.smem_eq m m' -> 
-      valid cs G (hemp m --> hemp m').
-      intros; goPropX. unfold hemp. eapply Imply_I.
-      generalize (Env cs0 ([|HT.semp m|]%PropX :: G) [|HT.semp m|]%PropX ).
-      intros. eapply Inj_E. eapply H0. left. reflexivity.
-      intros. rewrite H in H1. eapply Inj_I. auto.
-    Qed.
-
-    Definition emp : Hprop := Build_Hprop _ hemp_respects.
-*)
-
-    Definition star sos (l r : hprop sos) : hprop sos :=
-      fun m => PropX.Exists (fun ml : HT.smem => PropX.Exists (fun mr : HT.smem =>
-        PropX.And (PropX.Inj (HT.split m ml mr)) (And (l ml) (r mr)))).
-
-(*
-    Theorem hstar_respects (l r : Hprop) : forall cs G m m', HT.smem_eq m m' -> 
-      valid cs G ((hstar l r) m --> (hstar l r) m').
-    Proof.
-      intros; unfold hstar in *. eapply Imply_I. eapply Exists_E.
-      econstructor. left. reflexivity.
-      intros; eapply Exists_E. econstructor; left; reflexivity.
-      intros. eapply Exists_I. instantiate (1 := B). eapply Exists_I. instantiate (1 := B0).
-      repeat eapply And_I.
-      2: eapply And_E1; eapply And_E2; econstructor; left; reflexivity.
-      2: eapply And_E2; eapply And_E2; econstructor; left; reflexivity.
-      eapply Inj_E. eapply And_E1. econstructor. left. reflexivity.
-      intros. rewrite H in H0. eapply Inj_I; auto.
-    Qed.
-
-    Definition star (l r : Hprop) : Hprop := Build_Hprop _ (hstar_respects l r).
-*)
-      
-(*
-    Definition cptr sos (stateMem : stateType -> H.mem) (p : pcType) 
-      (t : stateType -> hprop sos) : hprop sos :=
-      fun h => 
-        PropX.And 
-          (emp h)
-          (PropX.Cptr p
-            (fun x : stateType => PropX.Exists (fun m => 
-              PropX.And (PropX.Inj (HT.satisfies m (stateMem x))) (t x m)))).
-    Theorem hcptr_respects (stateMem : stateType -> H.mem) (p : pcType) (t : stateType -> Hprop) : 
-      forall cs G m m', 
-        HT.smem_eq m m' -> valid cs G ((hcptr stateMem p t) m --> (hcptr stateMem p t) m').
-    Proof.
-      unfold hcptr; intros. eapply Imply_I. eapply And_I.
-      2: eapply And_E2; econstructor; left; reflexivity.
-      eapply Imply_E. 2: eapply And_E1; econstructor; left; reflexivity. eapply Imply_I.
-      generalize hemp_respects. intros. eapply H0 in H. eapply Imply_E. 2: eassumption.
-      unfold hemp in *. clear. eapply Imply_I. 
-      eapply Imply_E. econstructor; left; reflexivity. econstructor; right; left; reflexivity.
-    Qed.
-
-    Definition cptr (stateMem : stateType -> H.mem) (p : pcType) (t : stateType -> Hprop) : Hprop :=
-      Build_Hprop _ (hcptr_respects stateMem p t).
-*)
-    Definition ex sos (T : Type) (p : T -> hprop sos) : hprop sos :=
-      fun h => PropX.Exists (fun t => p t h).
-(*    
-    Definition hex_respects T (p : T -> Hprop) : forall cs G m m', 
-      HT.smem_eq m m' -> valid cs G ((hex _ p) m --> (hex _ p) m').
-    Proof.
-      unfold hex; intros. eapply Imply_I. eapply Exists_E. econstructor; left; reflexivity.
-      intros. eapply Exists_I. instantiate (1 := B). destruct (p B). simpl in *.
-        specialize (respects0 cs0 G _ _ H). generalize respects0. clear. intros.
-        eapply Imply_E. 2: econstructor; left; reflexivity.
-        eapply valid_weaken. eassumption. clear.
-        red. intros. simpl. tauto.
-    Qed.
-
-    Definition ex (T : Type) (p : T -> Hprop) : Hprop := Build_Hprop _ (hex_respects T p).
-*)
-
-    Definition hptsto sos (p : H.addr) (v : H.byte) : hprop sos :=
-      fun h => PropX.And (PropX.Inj (HT.smem_get p h = Some v))
-        (PropX.Forall (fun p' =>
-          (PropX.Imply (PropX.Inj (p <> p')) (PropX.Inj (HT.smem_get p' h = None))))).
-
-    (** Lemmas **)
+    Hint Immediate HT.split_comm : heaps.
+    Hint Resolve HT.split_assoc HT.disjoint_split_join HT.split_split_disjoint : heaps.
 
     Lemma himp_star_comm : forall P Q, himp (star P Q) (star Q P).
     Proof.
-      unfold star; doIt. apply Imply_I. eapply Exists_E. econstructor. left; auto.
-      intros. eapply Exists_E. econstructor; left; auto. intros.
-      do 2 eapply Exists_I. repeat eapply And_I.
-      2: eapply And_E2; eapply And_E2; econstructor; left; auto.
-      2: eapply And_E1; eapply And_E2; econstructor; left; auto.
-      eapply Imply_E. 2: eapply And_E1; econstructor; left; eauto.
-      eapply Imply_I. eapply Inj_E. econstructor; left; auto. intros.
-      apply HT.split_comm in H. apply Inj_I. auto.
+      unfold star; doIt; eauto with heaps. 
     Qed.      
 
     Theorem himp_star_comm_p : forall P Q R, himp (star P Q) R -> himp (star Q P) R.
     Proof.
-      doIt. generalize (himp_star_comm Q P). intros. eapply Imply_I. eapply Imply_E.
-      eapply interp_weaken in H. eassumption. specialize (H0 m).
-      eapply Imply_E. eapply interp_weaken in H0. eapply H0. econstructor; left; auto.
+      unfold star; doIt. eauto with heaps. 
     Qed.
     Theorem himp_star_comm_c : forall P Q R, himp R (star P Q) -> himp R (star Q P).
     Proof.
-    Admitted.
+      unfold star; doIt. eauto with heaps.
+    Qed.
 
     Theorem heq_star_comm : forall P Q R, heq (star P Q) R -> heq (star Q P) R.
     Proof.
@@ -236,123 +117,78 @@ Module SepTheoryX (H : Heap).
     Theorem himp_star_assoc_p : forall P Q R S,
       himp (star P (star Q R)) S -> himp (star (star P Q) R) S.
     Proof.
-(*
-      doIt. apply HT.split_comm. apply HT.split_comm in H. eapply HT.split_assoc; try eassumption. 
-      apply HT.split_comm. eassumption. eapply HT.disjoint_split_join.
-      apply HT.disjoint_comm. eapply HT.split_split_disjoint; eauto.
-      apply HT.split_comm in H0; eassumption.
-*)
-    Admitted.
+      doIt.
+      eapply HT.split_comm. eapply HT.split_assoc. eapply HT.split_comm. eassumption. eapply HT.split_comm. eassumption.
+      eapply HT.disjoint_split_join. eapply HT.disjoint_comm. eauto with heaps. 
+    Qed.
     Theorem himp_star_assoc_c : forall P Q R S, 
       himp S (star P (star Q R)) -> himp S (star (star P Q) R).
     Proof.
-(*
-      doIt. eapply HT.split_assoc; eassumption. apply HT.split_comm.
-      apply HT.disjoint_split_join. apply HT.disjoint_comm.
-      eapply HT.split_split_disjoint. apply HT.split_comm. eassumption. eassumption.
-*)
-    Admitted.
+      doIt. eapply HT.split_assoc. eassumption. eassumption.
+      eapply HT.split_comm. eapply HT.disjoint_split_join. eapply HT.disjoint_comm. eauto with heaps.
+    Qed.
 
     Theorem heq_star_assoc : forall P Q R S, 
       heq S (star P (star Q R)) -> heq S (star (star P Q) R).
     Proof.
-(*
-      intros. generalize (himp_star_assoc_p P Q R S). generalize (himp_star_assoc_c P Q R S).
+      intros. generalize (@himp_star_assoc_p P Q R S). generalize (@himp_star_assoc_c P Q R S).
       firstorder.
-*)
-    Admitted.
+    Qed.
 
-    Theorem himp_star_frame : forall P Q R S, himp P Q -> himp R S -> himp (star P R) (star Q S).
+    Theorem himp_star_frame : forall P Q R S, 
+      himp P Q -> himp R S -> himp (star P R) (star Q S).
     Proof.
-(*
-      unfold himp; simpl; intros;
-        repeat match goal with
-                 | [ H : _ -> _ |- _ ] => apply H; clear H
-                 | [ H : ?X -> _ , H' : ?X |- _ ] => apply H in H'; clear H
-               end; goPropX.
-      apply simplify_bwd in H2. apply simplify_bwd in H3. apply H in H2. apply H0 in H3. doIt.
-      assumption.
-*)
-    Admitted.
+      doIt. 2: eapply H; eassumption. 2: eapply H0; eassumption. auto.
+    Qed.
 
     Theorem heq_star_frame : forall P Q R S, heq P Q -> heq R S -> heq (star P R) (star Q S).
     Proof.
-(*
-      intros; generalize (himp_star_frame P Q R S). generalize (himp_star_frame Q P S R).
-      unfold heq in *. intuition.
-*)
-    Admitted.
+      doIt. eapply himp_star_frame; eauto. eapply himp_star_frame; eauto.
+    Qed.
 
     Theorem himp_star_emp_p : forall P Q, himp P Q -> himp (star emp P) Q.
     Proof.
-(*
-      unfold himp. intros. eapply H. unfold star in *. simpl in *.
-      goPropX. apply simplify_bwd in H2. destruct P. simpl in *.
-      eapply HT.split_semp in H1; eauto.
-      apply simplify_fwd.  eapply Imply_E.  2: eassumption. eapply respects0. symmetry; auto.
-*)
-    Admitted.
+      doIt. eapply HT.split_semp in H0; subst; auto.
+    Qed.
 
     Theorem himp_star_emp_p' : forall P Q, himp (star emp P) Q -> himp P Q.
     Proof.
-(*
-      unfold himp. intros. eapply H. unfold star in *. simpl in *.
-      goPropX. do 2 eexists. split. eapply HT.split_a_semp_a. split; eauto.
-      eapply HT.semp_smem_emp.
-*)
-    Admitted.
+      doIt. eapply HT.split_a_semp_a. auto. eapply HT.semp_smem_emp.
+    Qed.
 
     Theorem himp_star_emp_c : forall P Q, himp P Q -> himp P (star emp Q).
     Proof.
-(*
-      unfold himp. intros. eapply H in H0. unfold star in *. simpl in *.
-      goPropX. do 2 eexists. split. eapply HT.split_a_semp_a. split; eauto.
-      eapply HT.semp_smem_emp.
-*)
-    Admitted.
+      doIt; auto. eapply HT.split_a_semp_a. eapply HT.semp_smem_emp.
+    Qed.
 
     Theorem himp_star_emp_c' : forall P Q, himp P (star emp Q) -> himp P Q.
     Proof.
-(*
-      unfold himp. intros. eapply H in H0. unfold star in *. simpl in *.
-      goPropX. apply simplify_bwd in H2. destruct Q. simpl in *.
-      eapply HT.split_semp in H1; eauto.
-      apply simplify_fwd. unfold interp in *.
-      eapply Imply_E. eapply respects0. symmetry; eassumption. auto.
-*)
-    Admitted.
+      doIt; auto. eapply HT.split_semp in H1; subst; auto.
+    Qed.
 
     Theorem heq_star_emp : forall P Q, heq P Q -> heq (star emp P) Q.
     Proof.
-(*
       intros. unfold heq in *; intuition.
       eapply himp_star_emp_p. auto.
       eapply himp_star_emp_c. auto.
-*)
-    Admitted.
+    Qed.
 
     Theorem heq_star_emp' : forall P Q, heq (star emp P) Q -> heq P Q.
     Proof.
-(*
       intros. unfold heq in *; intuition.
       eapply himp_star_emp_p' in H0. auto.
       eapply himp_star_emp_c' in H1. auto.
-*)
-    Admitted.
+    Qed.
 
     Theorem himp_star_cancel : forall P Q R, himp Q R -> himp (star P Q) (star P R).
     Proof.
-(*
       intros. eapply himp_star_frame. reflexivity. auto.
-*)
-    Admitted.
+    Qed.
 
     Theorem heq_star_cancel : forall P Q R, heq Q R -> heq (star P Q) (star P R).
     Proof.
-(*
       intros. eapply heq_star_frame. reflexivity. auto.
-*)
-    Admitted.
+    Qed.
 
   End env.
 End SepTheoryX.
